use ConnMan in ShardClerk

external/Goose/github_com/mit_pdos/gokv/connman.v
@@ -12,6 +12,14 @@ Definition ConnMan := struct.decl [
   "making" :: mapT condvarRefT
 ].
 
+Definition MakeConnMan: val :=
+  rec: "MakeConnMan" <> :=
+    let: "c" := struct.alloc ConnMan (zero_val (struct.t ConnMan)) in
+    struct.storeF ConnMan "mu" "c" (lock.new #());;
+    struct.storeF ConnMan "rpcCls" "c" (NewMap (struct.ptrT rpc.RPCClient));;
+    struct.storeF ConnMan "making" "c" (NewMap condvarRefT);;
+    "c".
+
 Definition ConnMan__getClient: val :=
   rec: "ConnMan__getClient" "c" "host" :=
     let: "ret" := ref (zero_val (refT (struct.t rpc.RPCClient))) in
