src/goose_lang/typing.v
@@ -542,6 +542,8 @@ Section goose_lang.
     eauto.
   Qed.
 
+  (* FIXME: Being an expression, this is removed when [subst] is executed.
+     We should use a value instead, probably a thunk. *)
   Definition NewMap (t:ty) : expr := Alloc (zero_val (mapValT t)).
   (*
   Theorem NewMap_t t Γ : has_zero t -> Γ ⊢ NewMap t : mapT t.
